compiled_combines_deterministic

src/CFG/IMP2_Proc_to_CFG.thy
@@ -296,6 +296,178 @@ next
   then show ?case by auto
 qed
 
+
+subsection \<open>Combine determinism for compiled CFGs\<close>
+
+text \<open>
+  \<open>combines\<close> is a primitive field of an arbitrary \<^typ>\<open>cfg\<close>, but for CFGs produced by
+  \<^const>\<open>compile_prog\<close> the call node determines the whole combine tuple.  The exit component
+  is therefore not independent data in a compiled CFG --- it is the callee procedure's exit
+  node, recoverable from the call node --- even though the record stores it (denormalised for
+  the solver's node-indexed combine equation).  The proofs are forward range arithmetic on the
+  compiler counter; no reverse node-to-source lookup is used.
+\<close>
+
+text \<open>Every combine call node emitted by \<^const>\<open>compile\<close> lies in the counter range \<open>[n, n')\<close>.\<close>
+lemma compile_combines_call_range:
+  "compile \<Pi> lay c n = (n', en, ex, E, C)
+   \<Longrightarrow> (cc, ce, cr, cd) \<in> C \<Longrightarrow> n \<le> cc \<and> cc < n'"
+proof (induction c arbitrary: n n' en ex E C cc ce cr cd rule: com.induct)
+  case SKIP then show ?case by auto
+next
+  case (Assign x a) then show ?case by auto
+next
+  case (Seq c1 c2)
+  from Seq.prems(1) obtain n1 en1 ex1 E1 C1 n2 en2 ex2 E2 C2 where
+    c1: "compile \<Pi> lay c1 n = (n1, en1, ex1, E1, C1)"
+    and c2: "compile \<Pi> lay c2 n1 = (n2, en2, ex2, E2, C2)"
+    and n': "n' = n2" and C: "C = C1 \<union> C2"
+    by (auto split: prod.splits)
+  from Seq.prems(2) C consider "(cc, ce, cr, cd) \<in> C1" | "(cc, ce, cr, cd) \<in> C2" by auto
+  then show ?case
+  proof cases
+    case 1
+    from Seq.IH(1)[OF c1 this] compile_counter_mono[OF c2] n' show ?thesis by simp
+  next
+    case 2
+    from Seq.IH(2)[OF c2 this] compile_counter_mono[OF c1] n' show ?thesis by simp
+  qed
+next
+  case (If b c1 c2)
+  from If.prems(1) obtain n1 en1 ex1 E1 C1 n2 en2 ex2 E2 C2 where
+    c1: "compile \<Pi> lay c1 (Suc n) = (n1, en1, ex1, E1, C1)"
+    and c2: "compile \<Pi> lay c2 n1 = (n2, en2, ex2, E2, C2)"
+    and n': "n' = Suc n2" and C: "C = C1 \<union> C2"
+    by (auto split: prod.splits)
+  from If.prems(2) C consider "(cc, ce, cr, cd) \<in> C1" | "(cc, ce, cr, cd) \<in> C2" by auto
+  then show ?case
+  proof cases
+    case 1
+    from If.IH(1)[OF c1 this] compile_counter_mono[OF c2] n' show ?thesis by simp
+  next
+    case 2
+    from If.IH(2)[OF c2 this] compile_counter_mono[OF c1] n' show ?thesis by simp
+  qed
+next
+  case (While b c)
+  from While.prems(1) obtain n1 en1 ex1 E1 C1 where
+    c: "compile \<Pi> lay c (Suc n) = (n1, en1, ex1, E1, C1)"
+    and n': "n' = Suc n1" and C: "C = C1"
+    by (auto split: prod.splits)
+  from While.prems(2) C have "(cc, ce, cr, cd) \<in> C1" by simp
+  from While.IH[OF c this] n' show ?case by simp
+next
+  case (Scope c)
+  from Scope.prems(1) obtain n1 en1 ex1 E1 C1 where
+    c: "compile \<Pi> lay c (Suc n) = (n1, en1, ex1, E1, C1)"
+    and n': "n' = Suc n1" and C: "C = C1 \<union> {(n, ex1, n1, None)}"
+    by (auto split: prod.splits)
+  from Scope.prems(2) C consider "(cc, ce, cr, cd) \<in> C1" | "(cc, ce, cr, cd) = (n, ex1, n1, None)"
+    by auto
+  then show ?case
+  proof cases
+    case 1
+    from Scope.IH[OF c this] n' show ?thesis by simp
+  next
+    case 2
+    from compile_counter_mono[OF c] n' show ?thesis using \<open>(cc, ce, cr, cd) = (n, ex1, n1, None)\<close> by simp
+  qed
+next
+  case (Call dst p actuals)
+  from Call.prems show ?case by (auto split: option.splits prod.splits)
+next
+  case Restore then show ?case by auto
+qed
+
+text \<open>Within one \<^const>\<open>compile\<close> the call node determines the combine tuple.\<close>
+lemma compile_combines_functional:
+  "compile \<Pi> lay c n = (n', en, ex, E, C)
+   \<Longrightarrow> (cc, ce1, cr1, cd1) \<in> C \<Longrightarrow> (cc, ce2, cr2, cd2) \<in> C
+   \<Longrightarrow> (ce1, cr1, cd1) = (ce2, cr2, cd2)"
+proof (induction c arbitrary: n n' en ex E C cc ce1 cr1 cd1 ce2 cr2 cd2 rule: com.induct)
+  case SKIP then show ?case by auto
+next
+  case (Assign x a) then show ?case by auto
+next
+  case (Seq c1 c2)
+  from Seq.prems(1) obtain n1 en1 ex1 E1 C1 n2 en2 ex2 E2 C2 where
+    c1: "compile \<Pi> lay c1 n = (n1, en1, ex1, E1, C1)"
+    and c2: "compile \<Pi> lay c2 n1 = (n2, en2, ex2, E2, C2)"
+    and C: "C = C1 \<union> C2"
+    by (auto split: prod.splits)
+  have rng1: "\<And>e r d. (cc, e, r, d) \<in> C1 \<Longrightarrow> cc < n1"
+    using compile_combines_call_range[OF c1] by blast
+  have rng2: "\<And>e r d. (cc, e, r, d) \<in> C2 \<Longrightarrow> n1 \<le> cc"
+    using compile_combines_call_range[OF c2] by blast
+  from Seq.prems(2) C have m1: "(cc, ce1, cr1, cd1) \<in> C1 \<union> C2" by simp
+  from Seq.prems(3) C have m2: "(cc, ce2, cr2, cd2) \<in> C1 \<union> C2" by simp
+  from m1 m2 rng1 rng2 consider
+      "(cc, ce1, cr1, cd1) \<in> C1 \<and> (cc, ce2, cr2, cd2) \<in> C1"
+    | "(cc, ce1, cr1, cd1) \<in> C2 \<and> (cc, ce2, cr2, cd2) \<in> C2"
+    by (metis Un_iff linorder_not_le)
+  then show ?case
+  proof cases
+    case 1 thus ?thesis using Seq.IH(1)[OF c1] by blast
+  next
+    case 2 thus ?thesis using Seq.IH(2)[OF c2] by blast
+  qed
+next
+  case (If b c1 c2)
+  from If.prems(1) obtain n1 en1 ex1 E1 C1 n2 en2 ex2 E2 C2 where
+    c1: "compile \<Pi> lay c1 (Suc n) = (n1, en1, ex1, E1, C1)"
+    and c2: "compile \<Pi> lay c2 n1 = (n2, en2, ex2, E2, C2)"
+    and C: "C = C1 \<union> C2"
+    by (auto split: prod.splits)
+  have rng1: "\<And>e r d. (cc, e, r, d) \<in> C1 \<Longrightarrow> cc < n1"
+    using compile_combines_call_range[OF c1] by blast
+  have rng2: "\<And>e r d. (cc, e, r, d) \<in> C2 \<Longrightarrow> n1 \<le> cc"
+    using compile_combines_call_range[OF c2] by blast
+  from If.prems(2) C have m1: "(cc, ce1, cr1, cd1) \<in> C1 \<union> C2" by simp
+  from If.prems(3) C have m2: "(cc, ce2, cr2, cd2) \<in> C1 \<union> C2" by simp
+  from m1 m2 rng1 rng2 consider
+      "(cc, ce1, cr1, cd1) \<in> C1 \<and> (cc, ce2, cr2, cd2) \<in> C1"
+    | "(cc, ce1, cr1, cd1) \<in> C2 \<and> (cc, ce2, cr2, cd2) \<in> C2"
+    by (metis Un_iff linorder_not_le)
+  then show ?case
+  proof cases
+    case 1 thus ?thesis using If.IH(1)[OF c1] by blast
+  next
+    case 2 thus ?thesis using If.IH(2)[OF c2] by blast
+  qed
+next
+  case (While b c)
+  from While.prems(1) obtain n1 en1 ex1 E1 C1 where
+    c: "compile \<Pi> lay c (Suc n) = (n1, en1, ex1, E1, C1)"
+    and C: "C = C1"
+    by (auto split: prod.splits)
+  from While.prems(2,3) C While.IH[OF c] show ?case by simp
+next
+  case (Scope c)
+  from Scope.prems(1) obtain n1 en1 ex1 E1 C1 where
+    c: "compile \<Pi> lay c (Suc n) = (n1, en1, ex1, E1, C1)"
+    and C: "C = C1 \<union> {(n, ex1, n1, None)}"
+    by (auto split: prod.splits)
+  have rng: "\<And>e r d. (cc, e, r, d) \<in> C1 \<Longrightarrow> Suc n \<le> cc"
+    using compile_combines_call_range[OF c] by blast
+  from Scope.prems(2) C have m1: "(cc, ce1, cr1, cd1) \<in> C1 \<union> {(n, ex1, n1, None)}" by simp
+  from Scope.prems(3) C have m2: "(cc, ce2, cr2, cd2) \<in> C1 \<union> {(n, ex1, n1, None)}" by simp
+  from m1 m2 rng consider
+      "(cc, ce1, cr1, cd1) \<in> C1 \<and> (cc, ce2, cr2, cd2) \<in> C1"
+    | "(cc, ce1, cr1, cd1) = (n, ex1, n1, None) \<and> (cc, ce2, cr2, cd2) = (n, ex1, n1, None)"
+    by (metis Un_iff insertE singletonD Suc_n_not_le_n fst_conv)
+  then show ?case
+  proof cases
+    case 1 thus ?thesis using Scope.IH[OF c] by blast
+  next
+    case 2 thus ?thesis by simp
+  qed
+next
+  case (Call dst p actuals)
+  from Call.prems show ?case by (auto split: option.splits prod.splits)
+next
+  case Restore then show ?case by auto
+qed
+
 lemma compile_procs_bodies_finite:
   "compile_procs_bodies \<Pi> ps base_lay full_lay n = (n', full_lay', E, C)
    \<Longrightarrow> finite E \<and> finite C"
@@ -336,6 +508,164 @@ lemma compile_prog_finite:
        dest: compile_procs_list_finite compile_finite
        intro: finite_UnI)
 
+
+lemma compile_procs_bodies_counter_mono:
+  "compile_procs_bodies \<Pi> ps base_lay full_lay n = (n', full_lay', E, C) \<Longrightarrow> n \<le> n'"
+proof (induction ps arbitrary: full_lay n n' full_lay' E C)
+  case Nil then show ?case by auto
+next
+  case (Cons p ps)
+  show ?case
+  proof (cases "\<Pi> p")
+    case None
+    with Cons.prems have "compile_procs_bodies \<Pi> ps base_lay full_lay n = (n', full_lay', E, C)"
+      by simp
+    from Cons.IH[OF this] show ?thesis .
+  next
+    case (Some decl)
+    with Cons.prems obtain n1 en ex E0 C0 full_lay1 n2 full_lay2 Eacc Cacc where
+      cp: "compile \<Pi> base_lay (with_result (body decl) (result decl)) n = (n1, en, ex, E0, C0)"
+      and rest: "compile_procs_bodies \<Pi> ps base_lay full_lay1 n1 = (n2, full_lay2, Eacc, Cacc)"
+      and n': "n' = n2"
+      by (auto split: prod.splits option.splits)
+    from compile_counter_mono[OF cp] Cons.IH[OF rest] n' show ?thesis by simp
+  qed
+qed
+
+lemma compile_procs_bodies_combines_range:
+  "compile_procs_bodies \<Pi> ps base_lay full_lay n = (n', full_lay', E, C)
+   \<Longrightarrow> (cc, ce, cr, cd) \<in> C \<Longrightarrow> n \<le> cc \<and> cc < n'"
+proof (induction ps arbitrary: full_lay n n' full_lay' E C cc ce cr cd)
+  case Nil then show ?case by auto
+next
+  case (Cons p ps)
+  show ?case
+  proof (cases "\<Pi> p")
+    case None
+    with Cons.prems(1) have b: "compile_procs_bodies \<Pi> ps base_lay full_lay n = (n', full_lay', E, C)"
+      by simp
+    from Cons.IH[OF b Cons.prems(2)] show ?thesis .
+  next
+    case (Some decl)
+    with Cons.prems(1) obtain n1 en ex E0 C0 full_lay1 n2 full_lay2 Eacc Cacc where
+      cp: "compile \<Pi> base_lay (with_result (body decl) (result decl)) n = (n1, en, ex, E0, C0)"
+      and rest: "compile_procs_bodies \<Pi> ps base_lay full_lay1 n1 = (n2, full_lay2, Eacc, Cacc)"
+      and n': "n' = n2" and C: "C = C0 \<union> Cacc"
+      by (auto split: prod.splits option.splits)
+    from Cons.prems(2) C consider "(cc, ce, cr, cd) \<in> C0" | "(cc, ce, cr, cd) \<in> Cacc" by auto
+    then show ?thesis
+    proof cases
+      case 1
+      from compile_combines_call_range[OF cp 1] compile_procs_bodies_counter_mono[OF rest] n'
+      show ?thesis by simp
+    next
+      case 2
+      from Cons.IH[OF rest 2] compile_counter_mono[OF cp] n' show ?thesis by simp
+    qed
+  qed
+qed
+
+lemma compile_procs_bodies_combines_functional:
+  "compile_procs_bodies \<Pi> ps base_lay full_lay n = (n', full_lay', E, C)
+   \<Longrightarrow> (cc, ce1, cr1, cd1) \<in> C \<Longrightarrow> (cc, ce2, cr2, cd2) \<in> C
+   \<Longrightarrow> (ce1, cr1, cd1) = (ce2, cr2, cd2)"
+proof (induction ps arbitrary: full_lay n n' full_lay' E C cc ce1 cr1 cd1 ce2 cr2 cd2)
+  case Nil then show ?case by auto
+next
+  case (Cons p ps)
+  show ?case
+  proof (cases "\<Pi> p")
+    case None
+    with Cons.prems(1) have b: "compile_procs_bodies \<Pi> ps base_lay full_lay n = (n', full_lay', E, C)"
+      by simp
+    from Cons.IH[OF b Cons.prems(2) Cons.prems(3)] show ?thesis .
+  next
+    case (Some decl)
+    with Cons.prems(1) obtain n1 en ex E0 C0 full_lay1 n2 full_lay2 Eacc Cacc where
+      cp: "compile \<Pi> base_lay (with_result (body decl) (result decl)) n = (n1, en, ex, E0, C0)"
+      and rest: "compile_procs_bodies \<Pi> ps base_lay full_lay1 n1 = (n2, full_lay2, Eacc, Cacc)"
+      and C: "C = C0 \<union> Cacc"
+      by (auto split: prod.splits option.splits)
+    have rng0: "\<And>e r d. (cc, e, r, d) \<in> C0 \<Longrightarrow> cc < n1"
+      using compile_combines_call_range[OF cp] by blast
+    have rngA: "\<And>e r d. (cc, e, r, d) \<in> Cacc \<Longrightarrow> n1 \<le> cc"
+      using compile_procs_bodies_combines_range[OF rest] by blast
+    from Cons.prems(2) C have m1: "(cc, ce1, cr1, cd1) \<in> C0 \<union> Cacc" by simp
+    from Cons.prems(3) C have m2: "(cc, ce2, cr2, cd2) \<in> C0 \<union> Cacc" by simp
+    from m1 m2 rng0 rngA consider
+        "(cc, ce1, cr1, cd1) \<in> C0 \<and> (cc, ce2, cr2, cd2) \<in> C0"
+      | "(cc, ce1, cr1, cd1) \<in> Cacc \<and> (cc, ce2, cr2, cd2) \<in> Cacc"
+      by (metis Un_iff linorder_not_le)
+    then show ?thesis
+    proof cases
+      case 1 thus ?thesis using compile_combines_functional[OF cp] by blast
+    next
+      case 2 thus ?thesis using Cons.IH[OF rest] by blast
+    qed
+  qed
+qed
+
+lemma compile_procs_list_combines_range:
+  assumes "compile_procs_list \<Pi> ps lay n = (n', lay', E, C)"
+    and "(cc, ce, cr, cd) \<in> C"
+  shows "n \<le> cc \<and> cc < n'"
+proof -
+  from assms(1) obtain n0 base_lay where
+    b: "compile_procs_bodies \<Pi> ps base_lay lay n = (n', lay', E, C)"
+    unfolding compile_procs_list_def by (auto simp: Let_def split: prod.splits)
+  from compile_procs_bodies_combines_range[OF b assms(2)] show ?thesis .
+qed
+
+lemma compile_procs_list_combines_functional:
+  assumes "compile_procs_list \<Pi> ps lay n = (n', lay', E, C)"
+    and "(cc, ce1, cr1, cd1) \<in> C" and "(cc, ce2, cr2, cd2) \<in> C"
+  shows "(ce1, cr1, cd1) = (ce2, cr2, cd2)"
+proof -
+  from assms(1) obtain n0 base_lay where
+    b: "compile_procs_bodies \<Pi> ps base_lay lay n = (n', lay', E, C)"
+    unfolding compile_procs_list_def by (auto simp: Let_def split: prod.splits)
+  from compile_procs_bodies_combines_functional[OF b assms(2) assms(3)] show ?thesis .
+qed
+
+
+text \<open>
+  Headline: in a compiled CFG the call node determines the whole combine tuple.  In particular
+  the exit component --- the callee procedure's exit node --- is not independent data; it is a
+  function of the call node.  \<open>combines\<close> stays a primitive \<^typ>\<open>cfg\<close> field (denormalised for the
+  solver's node-indexed combine equation), but for \<^const>\<open>compile_prog\<close> outputs this theorem
+  records that the denormalisation is redundant.
+\<close>
+lemma compiled_combines_deterministic:
+  assumes "(cc, ce1, cr1, cd1) \<in> combines (compile_prog \<Pi> ps main)"
+      and "(cc, ce2, cr2, cd2) \<in> combines (compile_prog \<Pi> ps main)"
+  shows "(ce1, cr1, cd1) = (ce2, cr2, cd2)"
+proof -
+  obtain n1 lay Eproc Cproc where
+    procs: "compile_procs_list \<Pi> ps (\<lambda>_. None) 0 = (n1, lay, Eproc, Cproc)"
+    by (metis prod_cases4)
+  obtain n2 en ex Emain Cmain where
+    mainc: "compile \<Pi> lay main n1 = (n2, en, ex, Emain, Cmain)"
+    by (metis prod_cases5)
+  have comb: "combines (compile_prog \<Pi> ps main) = Cproc \<union> Cmain"
+    unfolding compile_prog_def compile_prog_with_regions_def
+    by (simp add: procs mainc mk_cfg_def Let_def)
+  have rP: "\<And>e r d. (cc, e, r, d) \<in> Cproc \<Longrightarrow> cc < n1"
+    using compile_procs_list_combines_range[OF procs] by blast
+  have rM: "\<And>e r d. (cc, e, r, d) \<in> Cmain \<Longrightarrow> n1 \<le> cc"
+    using compile_combines_call_range[OF mainc] by blast
+  from assms(1) comb have m1: "(cc, ce1, cr1, cd1) \<in> Cproc \<union> Cmain" by simp
+  from assms(2) comb have m2: "(cc, ce2, cr2, cd2) \<in> Cproc \<union> Cmain" by simp
+  from m1 m2 rP rM consider
+      "(cc, ce1, cr1, cd1) \<in> Cproc \<and> (cc, ce2, cr2, cd2) \<in> Cproc"
+    | "(cc, ce1, cr1, cd1) \<in> Cmain \<and> (cc, ce2, cr2, cd2) \<in> Cmain"
+    by (metis Un_iff linorder_not_le)
+  then show ?thesis
+  proof cases
+    case 1 thus ?thesis using compile_procs_list_combines_functional[OF procs] by blast
+  next
+    case 2 thus ?thesis using compile_combines_functional[OF mainc] by blast
+  qed
+qed
 subsection \<open>Executable examples\<close>
 
 value "cfg_entry (compile_prog (\<lambda>_. None) [] IMP2_Proc.com.SKIP)"
